theories/simulations/msim/WSimFacts.v
@@ -25,26 +25,28 @@ Section LAT.
   Qed.
 
   Lemma wsim_lat_img_to_hoare fsp body_s body_t fl_s fl_t msk scp ps pt st arg
+    (PHY: fspec_physical fsp)
     (EQIT: eqit eq false true
             (SB.sandbox true msk scp (body_s arg))
             (SB.sandbox true msk scp (SModTr.trans sp_none (body_t arg))))
     :
     ⊢
     wsim fl_s fl_t IstEq (∅,∅) ibot ibot _ _ (ist_with_eq IstEq) ps pt
-      (st, SB.sandbox true msk scp (SModTr.HoareFun (fsp_some (to_fspec fsp)) body_s arg))
+      (st, SB.sandbox true msk scp (SModTr.HoareFun (fsp_some fsp) body_s arg))
       (st, SB.sandbox true msk scp (SModTr.trans sp_none (lat_img false fsp (Ret ()) body_t arg))).
   Proof using.
     iIntros. iApply isim_wsim. iIntros "W". iApply isim_lat_img_to_hoare; et.
   Qed.
 
   Lemma wsim_lat_real_to_hoare fsp body_s body_t fl_s fl_t msk scp ps pt st arg
+    (PHY: fspec_physical fsp)
     (EQIT: eqit eq false true
             (SB.sandbox true msk scp (body_s arg))
             (SB.sandbox false msk scp (SModTr.trans sp_none (body_t arg))))
     :
     ⊢
     wsim fl_s fl_t IstEq (∅,∅) ibot ibot _ _ (ist_with_eq IstEq) ps pt
-      (st, SB.sandbox true msk scp (SModTr.HoareFun (fsp_some (to_fspec fsp)) body_s arg))
+      (st, SB.sandbox true msk scp (SModTr.HoareFun (fsp_some fsp) body_s arg))
       (st, SB.sandbox false msk scp (SModTr.trans sp_none (lat_real false fsp (Ret ()) body_t arg))).
   Proof using.
     iIntros. iApply isim_wsim. iIntros "W". iApply isim_lat_real_to_hoare; et.
